Complete reversibility proofs wrt halting
Using a simple halting characterization i.e. `fractran_terminates` for now.

theories/FRACTRAN/Utils/reversibility_facts.v
@@ -10,24 +10,6 @@ From Undecidability.FRACTRAN
 From Undecidability.Synthetic
      Require Import Definitions.
 
-Section ListFacts.
-
-  Lemma length_one_iff_singleton {X} (l : list X) : length l = 1 <-> exists x, l = [x].
-  Proof.
-    destruct l; simpl; split.
-    - intros H. congruence.
-    - intros [x H]. congruence.
-    - intros [=]. apply length_zero_iff_nil in H0. exists x. now rewrite H0.
-    - intros [y]. now inversion H.
-  Qed.
-
-  Lemma length_at_least_0 {X} (l : list X) : length l >= 0.
-  Proof.
-    induction l as [|a l IHl]; simpl; lia.
-  Qed.
-
-End ListFacts.
-
 (* Some facts about prime factors due to Andrej *)
 Section Prime_factors.
 
@@ -123,9 +105,10 @@ Section Prime_factors.
 
 End Prime_factors.
 
-Section Fractran_Facts.
+Section Fractran_facts.
 
-  Lemma fractran_step_zero y l (Hl : l <> nil) (Hlreg : fractran_regular l) :
+  (* If computation starts from 0, it will stay at 0 *)
+  Lemma fractran_step_zero_input y l (Hl : l <> nil) (Hlreg : fractran_regular l) :
     l /F/ 0 → y <-> y = 0.
   Proof.
     split.
@@ -138,52 +121,72 @@ Section Fractran_Facts.
       constructor. lia.
   Qed.
 
-  Lemma fractran_steps_zero x l (Hl : l <> nil) (Hlreg : fractran_regular l) :
+  Lemma fractran_compute_zero_input x l (Hl : l <> nil) (Hlreg : fractran_regular l) :
     forall n, fractran_steps l n 0 x <-> x = 0.
   Proof.
     induction n as [|n IHn]; simpl; [split; auto|]. split.
-    - intros [y [Hy Hs]]. apply IHn. apply fractran_step_zero in Hy; subst; auto.
+    - intros [y [Hy Hs]]. apply IHn. apply fractran_step_zero_input in Hy; subst; auto.
     - intros ->. exists 0. split; [|now apply IHn].
-      apply fractran_step_zero; auto.
+      apply fractran_step_zero_input; auto.
   Qed.
 
-  Corollary fractran_nstop_zero l (Hl : l <> nil) (Hlreg : fractran_regular l) :
+  (* A computation that starts from 0 does not terminate *)
+  Corollary fractran_nstop_zero_input l (Hl : l <> nil) (Hlreg : fractran_regular l) :
     ~ l /F/ 0 ↓.
   Proof.
-    intros [y [[n Hy] Hstop]]. apply fractran_steps_zero in Hy; subst; auto.
+    intros [y [[n Hy] Hstop]]. apply fractran_compute_zero_input in Hy; subst; auto.
     destruct l as [| (c,d) l]; subst; [congruence|].
     apply (Hstop 0). constructor. lia.
   Qed.
 
-  Corollary fractran_singleton_steps_zero x c d (Hd : d <> 0) :
-    forall n, fractran_steps [(c,d)] n 0 x <-> x = 0.
+  Lemma fractran_step_zero_num_1 d l s u (Hd : d <> 0) : (0,d) :: l /F/ s → u <-> u = 0.
   Proof.
-    apply fractran_steps_zero; [congruence|].
-    constructor; auto.
+    constructor; [|intros ->; now constructor].
+    inversion 1; subst; [lia|]. exfalso. apply H5. now exists 0.
   Qed.
 
-  Corollary fractran_singleton_nstop_zero c d (Hd : d <> 0) : ~ [(c,d)] /F/ 0 ↓.
+  Corollary fractran_nstop_zero_num_1 d l s : ~ (0,d) :: l /F/ s ↓.
   Proof.
-    apply fractran_nstop_zero; [congruence|].
-    apply Forall_cons; auto.
+    destruct d as [|d]; simpl; intros [y [_ Hs]]; apply (Hs 0); now constructor.
   Qed.
 
-  Lemma fractran_step_nzero x y c d (Hx : x <> 0) (Hc : c <> 0) (Hd : d <> 0) :
-    [(c,d)] /F/ x → y -> y <> 0.
+  Lemma fractran_nstop_zero_num_2 a b d l x : ~ (S a, b) :: (0, d) :: l /F/ x ↓.
   Proof.
-    inversion 1; subst.
-    - lia.
-    - inversion H6.
+    destruct (divides_dec (S a) b) as [[k Hd]|_]; intros [y [[_ _] Hs]].
+    - apply (Hs (k*y)). constructor. lia.
+    - destruct (divides_dec (S a*y) b) as [[k Hd]|Hd].
+      + apply (Hs k). constructor. lia.
+      + apply (Hs 0). apply in_fractran_1; auto.
+        now constructor.
   Qed.
 
-  Lemma fractran_singleton_ndiv_stop_S x c d (Hx : x <> 0) (Hc : c <> 0) (Hd : d <> 0) :
+  Lemma fractran_step_zero_den_1 c l s u : l /F/ s → u -> (c,0) :: l /F/ s → u.
+  Proof.
+    intros H. destruct c as [|c]; [now constructor|].
+    destruct s as [|s]; [now constructor|].
+    apply in_fractran_1; [|auto]. intros [k Hd]. lia.
+  Qed.
+
+  Lemma fractran_stop_zero_den_1 c s (Hc : c <> 0) : [(c, 0)] /F/ s ↓.
+  Proof.
+    destruct s as [|s]; simpl.
+    - exists 1. constructor.
+      + exists 1. simpl. exists 1. constructor; [|reflexivity].
+        now constructor.
+      + intros z H. inversion H; subst; [lia|inversion H6].
+    - exists (S s). constructor.
+      + now exists 0.
+      + intros z H. inversion H; subst; [lia|inversion H6].
+  Qed.
+
+  Lemma fractran_stop_ndiv_singleton x c d (Hx : x <> 0) (Hc : c <> 0) (Hd : d <> 0) :
     ~ divides d c -> [(c,d)] /F/ x ↓.
   Proof.
     intros Hndiv%prime_key_div'; [|exact Hc|exact Hd].
     destruct Hndiv as [p H]. revert Hx.
     induction on x as IH with measure (count_pow p (pred x)).
     intros Hx. destruct (fractran_step_dec [(c,d)] x) as [[y Hxy]|Hs].
-    - assert (Hy : y <> 0) by (apply (fractran_step_nzero x _ c d); auto).
+    - assert (Hy : y <> 0) by (inversion Hxy; subst; [lia|inversion H6]).
       inversion Hxy; subst.
       + specialize (H x y Hx Hy ltac: (lia)). specialize (IH y).
         apply IH in H as [y' [[n Hyy'] Hs']]; [|exact Hy]. exists y'. split; [|exact Hs'].
@@ -193,19 +196,41 @@ Section Fractran_Facts.
       exists 0. now simpl.
   Qed.
 
-  Lemma redundant_fractran_step l1 l2 l3 c1 d1 c2 d2 x y : divides d1 d2 ->
-    l1 ++ [(c1,d1)] ++ l2 ++ [(c2,d2)] ++ l3 /F/ x → y <-> l1 ++ [(c1,d1)] ++ l2 ++ l3 /F/ x → y.
+  Lemma fractran_step_suffix l x y : l /F/ x → y -> forall s, l ++ s /F/ x → y.
   Proof.
-  Admitted.
+    intros H. destruct s as [|(c,d) t]; [now rewrite app_nil_r|].
+    induction l as [|(p,q) l IHl]; [inversion H|].
+    inversion H; subst; [now constructor|].
+    rewrite <- app_comm_cons. apply in_fractran_1; [exact H5|].
+    apply IHl, H6.
+  Qed.
 
-  (* forall l, if l is not redundant -> length l >= 2 -> not_reversible l *)
-  (* forall l, length l >= 2 -> reversible l -> redundant_fractran l *)
+  Lemma fractran_compute_suffix l x y n :
+    fractran_steps l n x y -> forall s, fractran_steps (l ++ s) n x y.
+  Proof.
+    revert x. induction n as [|n IHn]; simpl; [easy|].
+    intros x [y' [Hy' Hs]] s. exists y'. constructor; [|now apply IHn].
+    now apply fractran_step_suffix.
+  Qed.
 
-End Fractran_Facts.
+  Lemma fractran_stop_inv_ndiv l x : fractran_stop l x -> Forall (fun '(a,b) => ~ divides b (a*x)) l.
+  Proof.
+    induction l as [|(c,d) t IHl]; intros H; [constructor|].
+    apply fractan_stop_cons_inv in H. destruct H as [H1 H2].
+    constructor; [auto|]. apply IHl, H2.
+  Qed.
+
+  Lemma fractran_step_prefix l s x y : fractran_stop l x -> s /F/ x → y -> (l ++ s) /F/ x → y.
+  Proof.
+    intros Hns%fractran_stop_inv_ndiv Hs. induction l as [|(c,d) t IHl]; simpl; [exact Hs|].
+    apply in_fractran_1.
+    - now apply Forall_inv in Hns.
+    - apply IHl. now apply Forall_inv_tail in Hns.
+  Qed.
+
+End Fractran_facts.
 
 Section Small_fractran_halt_dec.
-
-  Variable (c d : nat) (Hd : d <> 0).
 
   Lemma fractran_empty_halt_dec : decidable (fun x => [] /F/ x ↓).
   Proof.
@@ -214,53 +239,174 @@ Section Small_fractran_halt_dec.
     intros z H. inversion H.
   Qed.
 
-  Lemma fractran_singleton_halt_dec : decidable (fun x => [(c,d)] /F/ x ↓).
+  Lemma fractran_singleton_halt_dec_regular c d (Hd : d <> 0) :
+    decidable (fun x => [(c,d)] /F/ x ↓).
   Proof.
     exists (fun x => match x, c with
                        0, _ => false
                      | _, 0 => false
                      | _, _ => if divides_dec c d then false else true
                      end).
-    intros x. split.
-    - intros [y [[n Hy] Hstop]]. destruct x as [| x].
-      + apply fractran_steps_zero in Hy; subst; [|congruence|].
-        * specialize (Hstop 0). exfalso. apply Hstop. constructor. lia.
-        * apply Forall_cons; auto.
+    split.
+    - destruct x as [| x].
+      + intros H%fractran_nstop_zero_input; [auto|congruence|].
+        constructor; auto.
       + destruct c as [| c'] eqn:Hc.
-        * specialize (Hstop 0). exfalso. apply Hstop. constructor. lia.
+        * now intros H%fractran_nstop_zero_num_1.
         * destruct (divides_dec c d) as [[k Hk] | Hndiv] eqn:H; subst; [|now rewrite H].
-          exfalso. apply (Hstop (k*y)). constructor. lia.
+          intros [y [[n Hn] Hstop]]. exfalso. apply (Hstop (k*y)). constructor. lia.
     - destruct x as [| x]; [congruence|].
       destruct c as [| c'] eqn:Hc; [congruence|].
-      destruct (divides_dec c d) as [[k Hk] | Hndiv] eqn:H; subst.
-      + now rewrite H.
-      + intros _. apply fractran_singleton_ndiv_stop_S; auto.
+      destruct (divides_dec c d) as [[k Hk] | Hndiv] eqn:H; subst; [now rewrite H|].
+      intros _. apply fractran_stop_ndiv_singleton; auto.
+  Qed.
+
+  Lemma fractran_singleton_halt_dec c d : decidable (fun x => [(c,d)] /F/ x ↓).
+  Proof.
+    destruct d as [|d]; simpl.
+    - destruct c as [|c]; simpl.
+      + exists (fun _ => false). constructor; [|now intros].
+        now intros H%fractran_nstop_zero_num_1.
+      + exists (fun _ => true). constructor; [now intros|].
+        intros _. now apply fractran_stop_zero_den_1.
+    - apply fractran_singleton_halt_dec_regular. auto.
   Qed.
 
 End Small_fractran_halt_dec.
 
-Theorem fractran_halt_dec_le2 l (Hl : fractran_regular l) :
-  (length l = 0 \/ length l = 1) -> decidable (fun x => l /F/ x ↓).
-Proof.
-  intros [ H%length_zero_iff_nil | H%length_one_iff_singleton ]; subst.
-  - exact fractran_empty_halt_dec.
-  - destruct H as [(c,d) H]. subst. apply Forall_inv in Hl. simpl in Hl.
-    now apply fractran_singleton_halt_dec.
-Qed.
-
 Section Redundant_fractran.
 
-  Definition fractran_redundant (l : list (nat * nat)) := exists l1 l2 l3 c1 d1 c2 d2,
-    l = l1 ++ [(c1,d1)] ++ l2 ++ [(c2,d2)] ++ l3 /\ divides d1 d2.
+  (* for a/b, c/d the fraction c/d may be redundant (and removed) *)
+  Lemma redundant_spec a b c d :
+    is_gcd d c 1 -> divides b d ->
+    forall x, divides d (c*x) -> divides b (a*x).
+  Proof.
+    intros Hdc [k1 Hbd] x Hd.
+    apply (is_rel_prime_div _ Hdc) in Hd as [k2 ?].
+    exists (k1*k2*a). nia.
+  Qed.
+
+  Lemma fractran_step_redundant a b c d l :
+    is_gcd d c 1 -> divides b d ->
+    forall s t, (a,b) :: (c,d) :: l /F/ s → t <-> (a,b) :: l /F/ s → t.
+  Proof.
+    intros Hdc [k1 Hbd] s t. constructor.
+    - inversion 1; subst; [now constructor|].
+      inversion H6; subst.
+      + assert (Hd: divides (k1*b) (c*s)) by (exists t; lia).
+        apply (redundant_spec a b) in Hd; auto; [now exfalso|now exists k1].
+      + apply in_fractran_1; auto.
+    - inversion 1; subst; [now constructor|].
+      apply in_fractran_1; auto. apply in_fractran_1; auto.
+      intros Hd. apply H5. apply (redundant_spec _ _ c (k1*b)); auto. now exists k1.
+  Qed.
+
+  (* if the second fraction is not redundant, then the program is not reversible *)
+  Lemma fractran_step_contradict_reversible a b c d l :
+    is_gcd b a 1 -> ~ divides b d ->
+    exists (s t u : nat),
+      (a,b) :: (c,d) :: l /F/ s → u /\ (a,b) :: (c,d) :: l /F/ t → u /\ s <> t.
+  Proof.
+    intros Hba Hbd. exists (c*b), (a*d), (a*c).
+    constructor; [constructor; lia|].
+    constructor. apply in_fractran_1.
+    - intros Hb. now do 2 apply (is_rel_prime_div _ Hba) in Hb.
+    - constructor. lia.
+    - intros E. apply Hbd. apply (is_rel_prime_div _ Hba). now exists c.
+  Qed.
 
 End Redundant_fractran.
 
-Section Large_fractran_not_reversible.
+Definition fractran_reversible (l : list (nat * nat)) :=
+  forall s t u, l /F/ s → u -> l /F/ t → u -> s = t.
 
-  Variable (l : list (nat * nat)) (Hreg : fractran_regular l) (Hlen : length l > 1).
+Lemma fractran_reversible_neg (l : list (nat * nat)) :
+  (exists s t u, l /F/ s → u /\ l /F/ t → u /\ s <> t) -> ~ fractran_reversible l.
+Proof.
+  unfold fractran_reversible.
+  intros (s & t & u & Hsu & Htu & ?) Hrev. apply H, (Hrev _ _ u); auto.
+Qed.
 
-  Lemma large_fractran_not_reversible :
-    (forall s t u, l /F/ s → u -> l /F/ t → u -> s = t) -> fractran_redundant l.
-  Admitted.
+Lemma fractran_step_iff_reversible l1 l2 :
+  (forall s t, l1 /F/ s → t <-> l2 /F/ s → t) -> fractran_reversible l1 -> fractran_reversible l2.
+Proof.
+  unfold fractran_reversible.
+  intros H Hrev s t u Hsu%H Htu%H. now apply Hrev with (u:=u).
+Qed.
 
-End Large_fractran_not_reversible.
+Lemma fractran_step_iff_halt l1 l2 :
+  (forall s t, l1 /F/ s → t <-> l2 /F/ s → t) -> (forall x, l1 /F/ x ↓ -> l2 /F/ x ↓).
+Proof.
+  intros H x. intros [y [[n Hn] Hs]]. exists y. constructor.
+  - exists n. revert x Hn. induction n as [|n IHn]; simpl; auto.
+    intros x [y' [Hy' Hs']]. exists y'. constructor; [now apply H|now apply IHn].
+  - intros z Hs'. now apply (Hs z), H.
+Qed.
+
+Corollary fractran_step_iff_halt_dec l1 l2 :
+  (forall s t, l1 /F/ s → t <-> l2 /F/ s → t) ->
+  decidable (fun x => l1 /F/ x ↓) -> decidable (fun x => l2 /F/ x ↓).
+Proof.
+  intros H [f Hdec]. exists f. intros x.
+  assert (l2 /F/ x ↓ -> l1 /F/ x ↓) by now apply fractran_step_iff_halt.
+  constructor; intros; [now apply Hdec, H0|].
+  apply (fractran_step_iff_halt l1 l2); auto. now apply Hdec.
+Qed.
+
+Lemma fractran_reversible_halt_dec_cons a b c d l (Ha : a <> 0) (Hc : c <> 0) :
+  (forall y, length y < length ((a,b) :: (c,d) :: l) -> fractran_reversible y -> decidable (fun x => y /F/ x ↓))
+  -> fractran_reversible ((a,b) :: (c,d) :: l) -> decidable (fun x => (a,b) :: (c,d) :: l /F/ x ↓).
+Proof.
+  intros IH.
+  destruct (bezout_generalized a b) as (_ & _ & gab & _ & _ & Hgab & _).
+  apply is_gcd_rel_prime in Hgab. destruct Hgab as (na & nb & (Hna & Hnb & Hab)).
+  destruct (bezout_generalized c d) as (_ & _ & gcd & _ & _ & Hgcd & _).
+  apply is_gcd_rel_prime in Hgcd. destruct Hgcd as (nc & nd & (Hnc & Hnd & Hcd)).
+  pose (l2 := ((na,nb) :: (nc,nd) :: l)).
+  assert (H: forall s t, (a,b) :: (c,d) :: l /F/ s → t <-> (na,nb) :: (nc,nd) :: l /F/ s → t).
+  { intros s t. constructor.
+    - inversion 1; subst; [constructor; nia|].
+      apply in_fractran_1.
+      + contradict H5. destruct H5 as [k H5]. exists k. nia.
+      + inversion H6; subst; [constructor; nia|].
+        apply in_fractran_1; [|exact H8].
+        contradict H7. destruct H7 as [k H7]. exists k. nia.
+    - inversion 1; subst; [constructor; nia|].
+      apply in_fractran_1.
+      + contradict H5. destruct H5 as [k H5]. exists k. nia.
+      + inversion H6; subst; [constructor; nia|].
+        apply in_fractran_1; [|exact H8].
+        contradict H7. destruct H7 as [k H7]. exists k. nia.
+  }
+  intros Hrev%(fractran_step_iff_reversible _ l2); [|apply H].
+  apply (fractran_step_iff_halt_dec l2 _).
+  - intros s t. apply iff_sym, H.
+  - destruct (divides_dec nd nb) as [[k Hd]|Hd].
+    + pose (l3 := (na,nb) :: l).
+      apply (fractran_step_iff_reversible _ l3) in Hrev.
+      * apply (fractran_step_iff_halt_dec l3 _).
+        intros s t. apply iff_sym, fractran_step_redundant; [|now exists k].
+        now apply is_gcd_sym. apply IH; auto.
+      * intros s t. apply fractran_step_redundant; [|now exists k].
+        now apply is_gcd_sym.
+    + assert (Hr : ~ fractran_reversible l2).
+      { apply fractran_reversible_neg, fractran_step_contradict_reversible; auto.
+        now apply is_gcd_sym.
+      }
+      exfalso. now apply Hr.
+Qed.
+
+Theorem fractran_reversible_halt_dec (l : list (nat * nat)) :
+  fractran_reversible l -> decidable (fun x => l /F/ x ↓).
+Proof.
+  induction on l as IH with measure (length l).
+  destruct l as [|(a,b) l]; simpl; [intros _; apply fractran_empty_halt_dec|].
+  destruct l as [|(c,d) l]; simpl; [intros _; apply fractran_singleton_halt_dec|].
+  destruct a as [|a]; simpl.
+  - intros _. exists (fun _ => false). split; [|now intros].
+    now intros H%fractran_nstop_zero_num_1.
+  - destruct c as [|c]; simpl.
+    + intros _. exists (fun _ => false). constructor; [|now intros].
+      now intros H%fractran_nstop_zero_num_2.
+    + now apply fractran_reversible_halt_dec_cons.
+Qed.
